\documentclass[12pt]{scrartcl}
\usepackage{geometry}
\geometry{a2paper, left=30pt, top=2cm, bottom=2cm}
\usepackage[utf8]{inputenc}
\usepackage[german]{babel}
\usepackage[fleqn]{amsmath}
\usepackage{amsfonts}
\usepackage{amssymb}
\usepackage{color}
\usepackage{ebproof}
\usepackage{pdflscape}
\usepackage{tikz}
\usepackage{xcolor}
\usepackage{mathrsfs}
\usepackage{marvosym}
\usepackage{ebproof}

\begin{document}

\begin{center}
	\huge\textbf{Exersice Sheet 7}\\[0.5cm]
	
	\Large
	$\mathrel{\vcenter{\hbox{\rule{2cm}{0.5pt}}}}$ \textbf{Sample 				Solution} $\mathrel{\vcenter{\hbox{\rule{2cm}{0.5pt}}}}$\\[1cm]
\end{center}
	\large
	
	\setlength{\marginparwidth}{0pt}
	
	\section*{Task 1: Partial Correctness}
	
	\subsection*{(a)}
	
	\begin{enumerate}
	\item[] $p:=2;$\\
			$q:=n-p;$\\
			$\text{\textbf{while}}\;\neg\text{\textbf{prime}}\left(p\right)\vee\neg\text{\textbf{prime}}\left(q\right)\;\text{\textbf{do}}$
			\begin{enumerate}
			\item[] $p:=p+1;$\\
					$q:=n-p;$
			\end{enumerate}
	\item[] $\text{\textbf{end}}$
	\end{enumerate}

	\subsection*{(b)}
	
	\pagenumbering{gobble}
	
	\normalsize
	
	\begin{enumerate}
	\item[] Let $c=\text{\textbf{while}}\;\neg\text{\textbf{prime}}\left(p\right)\vee\neg\text{\textbf{prime}}\left(q\right)\;\text{\textbf{do}}$
			\begin{enumerate}
			\item[] $p:=p+1;$\\
					$q:=n-p;$
			\end{enumerate}
	\item[] $\text{\textbf{end}}$
	\end{enumerate}		
	
	\begin{center}
	\begin{prooftree}
	\hypo {\textcircled{a}}
	\hypo {\textcircled{b}}
	\hypo {\textcircled{c}}
	\infer[left label = \small{(seq)}]2 {\left\{p=2\right\}\;q=n-p;\;c\;\left\{\text{\textbf{prime}}\left(p\right)\wedge\text{\textbf{prime}}\left(q\right)\wedge n=q+p\right\}}
	\infer[left label = \small{(seq)}]2 {\left\{\text{\textbf{true}}\right\}\;p:=2;\;q=n-p;\;c\left\{\text{\textbf{prime}}\left(p\right)\wedge\text{\textbf{prime}}\left(q\right)\wedge n=q+p\right\}}
	\end{prooftree}\vspace{1cm}
	\end{center}
	
	\textcircled{a}\\
	\begin{center}
	\begin{prooftree}
		\hypo {\models\left(\text{\textbf{true}}\Rightarrow 2=2\right)}
		\infer[left label = \small{(asgn)}]0 {\left\{2=2\right\}\;p:=2;\;\left\{p=2\right\}}
		\hypo {\models\left(p=2\Rightarrow p=2\right)}
		\infer[left label = \small{(cons)}]3 {\left\{\text{\textbf{true}}\right\}\;p:=2;\;\left\{p=2\right\}}
	\end{prooftree}\vspace{1cm}
	\end{center}
	
	\textcircled{b}\\
	\begin{center}
	\begin{prooftree}
		\hypo {\models\left(p=2\Rightarrow n-p=n-p\right)}
		\infer[left label = \small{(asgn)}]0 {\left\{n-p=n-p\right\}\;q:=n-p;\;\left\{q=n-p\right\}}
		\hypo {\models\left(q=n-p\Rightarrow q=n-p\right)}
		\infer[left label = \small{(cons)}]3 {\left\{p=2\right\}\;q=n-p;\;\left\{q=n-p\right\}}
	\end{prooftree}
	\end{center}\vspace{1cm}
	
	\textcircled{c}\\
	\begin{center}
	\begin{prooftree}
		\hypo {\models\left(q=n-p\Rightarrow n=q+p\right)}
		\hypo {\textcircled{d}}
		\infer[left label = \small{(while)}]1 {\left\{n=q+p\right\}\;c\;\left\{\text{\textbf{prime}}\left(p\right)\wedge\text{\textbf{prime}}\left(q\right)\wedge n=q+p\right\}}
		\hypo {\models\left(\left(\text{\textbf{prime}}\left(p\right)\wedge\text{\textbf{prime}}\left(q\right)\wedge n=q+p\right)\Rightarrow\left(\text{\textbf{prime}}\left(p\right)\wedge\text{\textbf{prime}}\left(q\right)\wedge n=q+p\right)\right)}
		\infer[left label = \small{(cons)}]3 {\left\{q=n-p\right\}\;c\;\left\{\text{\textbf{prime}}\left(p\right)\wedge\text{\textbf{prime}}\left(q\right)\wedge n=q+p\right\}}
	\end{prooftree}
	\end{center}\vspace{1cm}
	
	\textcircled{d}\\
	\begin{center}
	\begin{prooftree}
		\hypo {\models\left(n=q+p\wedge\left(\neg\text{\textbf{prime}}\left(p\right)\vee\neg\text{\textbf{prime}}\left(q\right)\right)\Rightarrow p+1=p+1\right)}
		\infer[left label = \small{(asgn)}]0 {\left\{p+1=p+1\right\}\;p:=p+1\;\left\{p=p+1\right\}}
		\hypo {\textcircled{e}}
		\infer[left label = \small{(seq)}]2 {\left\{p+1=p+1\right\}\;p:=p+1;\;q:=n-p;\;\left\{n=q+p\right\}}
		\hypo {\models\left(n=q+p\Rightarrow n=q+p\right)}
		\infer[left label = \small{(cons)}]3 {\left\{n=q+p\wedge\left(\neg\text{\textbf{prime}}\left(p\right)\vee\neg\text{\textbf{prime}}\left(q\right)\right)\right\}\;p:=p+1;\;q:=n-p;\;\left\{n=q+p\right\}}
	\end{prooftree}
	\end{center}\vspace{1cm}
	
	\textcircled{e}\\
	\begin{center}
	\begin{prooftree}
	\hypo {\models\left(p=p+1\Rightarrow n-p=n-p\right)}
	\infer[left label = (asgn)]0 {\left\{n-p=n-p\right\}\;q:=n-p\;\left\{q=n-p\right\}}
	\hypo {\models\left(q=n-p\Rightarrow n=q+p\right)}
	\infer[left label = \small{(cons)}]3 {\left\{p=p+1\right\}\;q:=n-p\;\left\{n=q+p\right\}}
	\end{prooftree}
	\end{center}\vspace{3cm}
	
	\section*{Task 2: Total Correctness}
	
	\subsection*{(a)}
	
	\begin{center}
	\begin{prooftree}
	\hypo {\models\left(\text{\textbf{true}}\Rightarrow\text{\textbf{true}}\right)}
	\hypo {\models\left(\left(\text{\textbf{true}}\wedge x\neq 0\right)\Rightarrow\text{\textbf{true}}\right)}
	\infer0 {\left\{\text{\textbf{true}}\right\}\;x:=x-1\;\left\{\text{\textbf{true}}\right\}}
	\hypo {\models\left(\text{\textbf{true}}\Rightarrow\text{\textbf{true}}\right)}
	\infer[left label = \small{(cons)}]3 {\left\{\text{\textbf{true}}\wedge x\neq 0\right\}\;x:=x-1\;\left\{\text{\textbf{true}}\right\}}
	\infer[left label = \small{(while)}]1 {\left\{\text{\textbf{true}}\right\}\;\text{\textbf{while}}\;x\neq 0\;\text{\textbf{do}}\;x:=x-1\;\text{\textbf{end}}\;\left\{\text{\textbf{true}}\wedge x=0\right\}}
	\hypo {\models\left(\left(x=0\wedge\text{\textbf{true}}\right)\Rightarrow\text{\textbf{true}}\right)}
	\infer[left label = \small{(cons)}]3 {\left\{\text{\textbf{true}}\right\}\;\text{\textbf{while}}\;x\neq 0\;\text{\textbf{do}}\;x:=x-1\;\text{\textbf{end}}\;\left\{\text{\textbf{true}}\right\}}
	\end{prooftree}
	\end{center}\vspace{1cm}
	
	\subsection*{(b)}
	
	\begin{center}
	\begin{prooftree}
	\hypo {\models\left(x>0\Rightarrow\left(\exists i\geq 0\wedge x=i\right)\right)}
	\hypo {\models\left(\left(i\geq 0\wedge x=i+1\right)\Rightarrow x\neq 0\right)}
	\hypo {\models\left(\left(i\geq 0\wedge x=i+1\right)\Rightarrow x=i+1\right)}
	\infer0 {\left\{x=i+1\right\}\;x:=x-1\;\left\{\Downarrow x=i\right\}}
	\hypo {\models\left(x=i\Rightarrow x=i\right)}
	\infer[left label = \small{(cons)}]3 {\left\{i\geq 0\wedge x=i+1\right\}\;x:=x-1\;\left\{\Downarrow x=i\right\}}
	\hypo {\left(x=0\Rightarrow x=0\right)}
	\infer[left label = \small{(while)}]3 {\left\{\exists i\geq 0\wedge x=i\right\}\;\text{\textbf{while}}\;x\neq 0\;\text{\textbf{do}}\;x:=x-1\;\text{\textbf{end}}\;\left\{\Downarrow x=0\right\}}
	\hypo {\left(x=0\Rightarrow\text{\textbf{true}}\right)}
	\infer[left label = \small{(cons)}]3 {\left\{x>0\right\}\;\text{\textbf{while}}\;x\neq 0\;\text{\textbf{do}}\;x:=x-1\;\text{\textbf{end}}\;\left\{\Downarrow\text{\textbf{true}}\right\}}
	\end{prooftree}
	\end{center}\vspace{1cm}
	
	\subsection*{(c)}
	
	This statement will be disproved by contradiction.\\
	
	\begin{center}
	\begin{prooftree}
	\hypo {\models\left(x<0\Rightarrow x< 0\right)}
	\hypo {\models\left(\left(x< 0\wedge x\neq 0\right)\Rightarrow x<0\right)}
	\hypo {\models\left(x<0\Rightarrow x<1\right)}
	\infer0 {\left\{x<1\right\}\;x:=x-1\;\left\{x<0\right\}}
	\hypo {\models\left(x<0\Rightarrow x<0\right)}
	\infer[left label = \small{(cons)}]3 {\left\{x<0\right\}\;x:=x-1\;\left\{x<0\right\}}
	\hypo {\models\left(x<0\Rightarrow x<0\right)}
	\infer[left label = \small{(cons)}]3 {\left\{x< 0\wedge x\neq 0\right\}\;x:=x-1\;\left\{x<0\right\}}
	\infer[left label = \small{(while)}]1 {\left\{x< 0\right\}\;\text{\textbf{while}}\;x\neq 0\;\text{\textbf{do}}\;x:=x-1\;\text{\textbf{end}}\;\left\{x<0\wedge x=0\right\}}
	\hypo {\models\left(\left(x=0\wedge x<0\right)\Rightarrow\text{\textbf{false}}\right)}
	\infer[left label = \small{(cons)}]3 {\left\{x<0\right\}\;\text{\textbf{while}}\;x\neq 0\;\text{\textbf{do}}\;x:=x-1\;\text{\textbf{end}}\;\left\{\text{\textbf{false}}\right\}}
	\end{prooftree}
	\end{center}
	
	As this statement holds the total correctness of $\left\{\text{\textbf{true}}\right\}\;\text{\textbf{while}}\;x\neq 0\;\text{\textbf{do}}\;x:=x-1\;\text{\textbf{end}}\;\left\{\Downarrow\text{\textbf{true}}\right\}$ is not satisfied.
	
	

\end{document}