\documentclass[12pt]{scrartcl}
\usepackage[utf8]{inputenc}
\usepackage[german]{babel}
%\usepackage[T1]{fontenc}
\usepackage{amsmath}
\usepackage{amsfonts}
\usepackage{amssymb}
\usepackage{color}
\usepackage{ebproof}
\usepackage{pdflscape}



\newcommand{\eRelation}[2]{$\dfrac{\text{#1}}{\text{#2}}$}
\newcommand{\eState}[2]{$\left\langle \text{#1},\; \text{#2}\right\rangle$}
\newcommand{\eRule}[3]{\eState{#1}{#2} $\rightarrow$ #3}

\newcommand{\lbr}{[\![}
\newcommand{\rbr}{]\!]}
\newcommand{\Tf}{\mathfrak{T}}
\newcommand{\lo}{\text{\textbf{loop}}}
\newcommand{\beg}{\text{\textbf{begin}}}
\newcommand{\en}{\text{\textbf{end}}}
\newcommand{\rep}{\text{\textbf{repeat}}}
\newcommand{\un}{\text{\textbf{until}}}
\newcommand{\jmp}{\text{\textbf{JMP}}}
\newcommand{\jmpf}{\text{\textbf{JMPF}}}
\newcommand{\loa}{\text{\textbf{LOAD}}}
\newcommand{\sto}{\text{\textbf{STO}}}
\newcommand{\pus}{\text{\textbf{PUSH}}}
\newcommand{\gt}{\text{\textbf{GT}}}
\newcommand{\sub}{\text{\textbf{SUB}}}

\usepackage[left=2cm,right=2cm,top=2cm,bottom=2cm]{geometry}
\begin{document}

\begin{center}
	\huge\textbf{Exersice Sheet 3}\\[0.5cm]
	
	\Large
	$\mathrel{\vcenter{\hbox{\rule{2cm}{0.5pt}}}}$ \textbf{Sample 				Solution} $\mathrel{\vcenter{\hbox{\rule{2cm}{0.5pt}}}}$\\[1cm]
\end{center}
	\large

	\section*{Task 1: Operational Equivalence}
	
	\indent\indent Prove or disprove:
	\begin{center}
		$\text{\textbf{repeat}}\; c\; \text{\textbf{until}}\; b \sim c;\; \text{\textbf{while}}\; b\; \text{\textbf{do}}\; c\; \text{\textbf{end}}$
	\end{center}
	\indent\indent The claim will be disproved using a counter example.\\\\
	\indent Lets assume $b:=\text{\textbf{true}}$ and $c:=\text{\textbf{skip}}$.\\
	\indent The \textbf{repeat} statement will terminate after the first iteration with\\\indent \eRule{$\text{\textbf{repeat}}\; c\; \text{\textbf{until}}\; b$}{$\sigma$}{$\sigma$} while the \textbf{while} statement will never terminate as \indent its condition is always satisfied.
	
	\rule{17cm}{0.4pt}\vspace{1cm}
	
	\indent Prove or disprove:
	\begin{center}
		$\underbrace{\text{\textbf{repeat}}\; c\; \text{\textbf{until}}\; b}_{=r} \sim c;\;\underbrace{\text{\textbf{while}}\; \neg b\; \text{\textbf{do}}\; c\; \text{\textbf{end}}}_{=w}$
	\end{center}
	
	\indent To prove this statement we claim that\\\indent $\left\langle r,\; \sigma\right\rangle\rightarrow\sigma^{'}\Leftrightarrow\left\langle c;\; w,\; \sigma\right\rangle\rightarrow\sigma^{'}$\\\\
	\indent $"\Rightarrow"$\\
	\indent\indent Proof by induction on the structure of proof trees\\\indent\indent $\left\langle \rep\; c\; \un\; b,\; \sigma\right\rangle\rightarrow\sigma^{'}$
	
	\subsection*{\quad Induction Base: {\boldmath ($b=\text{\textbf{true}}$)}}
		
	\begin{center}
		\begin{prooftree}
			\hypo{\cdots}
			\infer1{\left\langle c,\;\sigma\right\rangle\rightarrow\sigma^{'}}
			\hypo{\cdots}
			\infer1{\left\langle b,\;\sigma1^{'}\right\rangle\rightarrow\text{\textbf{true}}}
			\infer2[\small{(repeat-true)}]{\left\langle r,\;\sigma\right\rangle\rightarrow\sigma^{'}}
		\end{prooftree}
	\end{center}
	
	\indent\indent Applying this assignment to the \textbf{while}-sequence we receive:
	
	\begin{center}
		\begin{prooftree}
			\hypo{\left\langle c,\;\sigma\right\rangle\rightarrow\sigma^{'}}
			\hypo{\left\langle b,\;\sigma^{'}\right\rangle\rightarrow\text{\textbf{true}}}
			\infer1{\left\langle \neg b,\;\sigma^{'}\right\rangle\rightarrow\text{\textbf{false}}}
			\infer1[\small{(while-false)}]{\left\langle w,\;\sigma^{'}\right\rangle\rightarrow\sigma^{'}}
			\infer2[\small{(seq)}]{\left\langle c;\; w,\;\sigma\right\rangle\rightarrow\sigma^{'}}
		\end{prooftree}
	\end{center}
	
	Thus the claim holds if $b=\text{\textbf{true}}$.
	
	\subsection*{\quad Induction Hypothesis:}
	
	\indent\indent\indent $\left\langle r,\;\sigma^{'}\right\rangle\rightarrow\sigma^{''}\Rightarrow\left\langle c;\; w,\;\sigma^{'}\right\rangle\rightarrow\sigma^{''}$ holds.
	
	\subsection*{\quad Induction step: {\boldmath ($b=\text{\textbf{false}}$)}}
	
	\begin{center}
		\begin{prooftree}
			\hypo{\small{\text{\textbf{assumption}}}}
			\infer1{\left\langle c,\; \sigma\right\rangle\rightarrow\sigma^{'}}
			\hypo{\left\langle b,\; \sigma^{'}\right\rangle\rightarrow\text{\textbf{false}}}
			\hypo{\small{\text{\textbf{by assumption}}}}
			\infer1{\left\langle r,\; \sigma^{'}\right\rangle\rightarrow\sigma^{''}}
			\infer3[\small{(repeat-false)}]{\left\langle r,\; \sigma\right\rangle\rightarrow\sigma^{''}}
		\end{prooftree}
	\end{center}
	
	\indent\indent Applying the same assignment to the \textbf{while}-sequence we receive:
	
	\begin{center}
		\begin{prooftree}
			\hypo{\small{\text{\textbf{assumption}}}}
			\infer1{\left\langle c,\; \sigma\right\rangle\rightarrow\sigma^{'}}
			\hypo{\left\langle b,\; \sigma^{'}\right\rangle\rightarrow\text{\textbf{false}}}
			\infer1{\left\langle \neg b,\; \sigma^{'}\right\rangle\rightarrow\text{\textbf{true}}}
			\hypo{\text{\textbf{I.H.}}}
			\infer1{\left\langle c;\; w,\; \sigma^{'}\right\rangle\rightarrow\sigma^{''}}
			\infer1[!]{\left\langle c,\; \sigma^{'}\right\rangle\rightarrow\sigma^{'''} \quad \left\langle w,\; \sigma^{'''}\right\rangle\rightarrow\sigma^{''}}
			\infer2{\left\langle w,\; \sigma^{'}\right\rangle\rightarrow\sigma^{''}}
			\infer2{\left\langle c;\; w,\; \sigma\right\rangle\rightarrow\sigma^{''}}
		\end{prooftree}
	\end{center}
	
	\indent\indent Thus the claim also holds for $b=\text{\textbf{false}}$.\\\\
	\indent $"\Leftarrow"$ analogously.
	
	\section*{Task 2: Translation of Statements}

		\begin{center}
			$\Tf_{c}\lbr\rep\;c\;\un\;b\rbr =\Tf_{c}\lbr c\rbr ;\;\Tf_{b}\lbr b\rbr ;\; \jmpf\left(-|\Tf_{c}\lbr c\rbr |+|\Tf_{b}\lbr b\rbr |\right)$
		\end{center}
		
	\section*{Task 3: loop Loops}
	
	\subsection*{(a)}
	
		
	
	\normalsize
	\begin{center}
		\begin{prooftree}
			\hypo{\left\langle x > 0,\; \sigma\right\rangle\rightarrow\text{\textbf{false}}}
			\infer1{\left\langle \text{\textbf{loop}}\; x\; \text{\textbf{begin}}\; c\; \text{\textbf{end}},\; \sigma\right\rangle\rightarrow\sigma}
		\end{prooftree}
	\end{center}
	
	\begin{center}
		\begin{prooftree}
			\hypo{\left\langle x > 0,\; \sigma\right\rangle\rightarrow\text{\textbf{true}}}
			\hypo{\left\langle c,\;\sigma\right\rangle\rightarrow\sigma^{'}}
			\hypo{\left\langle z:=x-1,\;\sigma^{'}\right\rangle\rightarrow\sigma^{''}}
			\hypo{\left\langle \text{\textbf{loop}}\; z\; \text{\textbf{begin}}\; c\; \text{\textbf{end}},\; \sigma^{''}\right\rangle\rightarrow\sigma^{'''}}
			\infer4{\left\langle \text{\textbf{loop}}\; x\; \text{\textbf{begin}}\; c\; \text{\textbf{end}},\; \sigma\right\rangle\rightarrow\sigma^{'''}}
		\end{prooftree}
	\end{center}
	
	\large
	
	\subsection*{(b)}
	
	\begin{flalign}
		\nonumber & \Tf_{c}\lbr \lo\; x\;\beg\; c\;\en\rbr=\loa (x);\; \sto (\xi);\\ \nonumber & \loa (\xi);\; \pus (0);\; \gt ;\; \jmpf (|\Tf_{c}\lbr c\rbr |+6);\\ \nonumber & \Tf_{c}\lbr c\rbr ;\; \loa (\xi);\; \pus (1);\; \sub ;\; \sto (\xi);\; \jmp (-(|\Tf_{c}\lbr c\rbr | + 8))
	\end{flalign}
	
\end{document}